<?xml version="1.0"?>
<?xml-stylesheet type="text/xsl" href="owl2html.xsl"?>
<rdf:RDF 
     xml:base="fedora"
     xmlns:rdfs="http://www.w3.org/2000/01/rdf-schema#"
     xmlns:owl="http://www.w3.org/2002/07/owl#"
     xmlns:xsd="http://www.w3.org/2001/XMLSchema#"
     xmlns:rdf="http://www.w3.org/1999/02/22-rdf-syntax-ns#">
    <owl:Ontology rdf:about="http://fedora.info/definitions/v4/oai-pmh#">
        <rdfs:label xml:lang="en">Fedora Commons OAI-PMH Ontology</rdfs:label>
        <rdfs:comment xml:lang="en">Describes relationships between Fedora Commons Repository objects used to provide an OAI-PMH service.</rdfs:comment>
    </owl:Ontology>

    <owl:ObjectProperty rdf:about="http://fedora.info/definitions/v4/oai-pmh#isPartOfOAISet">
        <rdfs:comment xml:lang="en">Links a Fedora object to an OAI set.</rdfs:comment>
        <rdfs:domain rdf:resource="http://fcrepo.org/repository#object"/>
        <rdfs:range rdf:resource="http://fedora.info/definitions/v4/repository#resource"/>
    </owl:ObjectProperty>
    <owl:ObjectProperty rdf:about="http://fedora.info/definitions/v4/oai-pmh#hasOAISet">
        <rdfs:comment xml:lang="en">Adds new OAI Set definitions to a specialized parent object linking to all existing OAI Sets.</rdfs:comment>
        <rdfs:range rdf:resource="http://fedora.info/definitions/v4/repository#resource"/>
    </owl:ObjectProperty>
    <owl:ObjectProperty rdf:about="http://fedora.info/definitions/v4/oai-pmh#hasOaiDCRecord">
        <rdfs:comment xml:lang="en">Links to an oai_dc record emitted for the linked subject.</rdfs:comment>
        <rdfs:range rdf:resource="http://fedora.info/definitions/v4/repository#resource"/>
    </owl:ObjectProperty>
    <owl:DatatypeProperty rdf:about="http://fedora.info/definitions/v4/oai-pmh#hasOAISetName">
        <rdfs:comment xml:lang="en">The name of an OAI Set.</rdfs:comment>
        <rdfs:range rdf:resource="http://www.w3.org/2001/XMLSchema#string"/>
    </owl:DatatypeProperty>
    <owl:DatatypeProperty rdf:about="http://fedora.info/definitions/v4/oai-pmh#hasOAISetSpec">
        <rdfs:comment xml:lang="en">The SetSpec of an OAI Set.  See http://www.openarchives.org/OAI/openarchivesprotocol.html#Set</rdfs:comment>
        <rdfs:range rdf:resource="http://www.w3.org/2001/XMLSchema#string"/>
    </owl:DatatypeProperty>

</rdf:RDF>
